theories/iSL/Lazy.v
@@ -1,0 +1,3 @@
+Definition Lazy T := unit -> T.
+Notation "'lazy' x" := (fun _ : unit => x) (x at next level, at level 50).
+Notation "'force' x" := (x tt) (x at next level, at level 50).
